state equivalences between semantics

VerseRocq/verse/densem/densem.v
@@ -31,16 +31,16 @@ Open Scope mini_expr_scope.
 Open Scope env_scope.
 Open Scope set_scope.
 
+Lemma not_Singleton_empty : forall A B (x:B), ⌈ x ⌉ ≃ ∅ -> A.
+Admitted.
+
+
 (* --------------------------------------------------- *)
 
 Definition VAL := P value.
 Definition ENV := P env.
 
-Definition guard {A} (ϕ : Prop) (e : P A) : P A := 
-  fun ρ => ϕ /\ (ρ ∈ e).
-
-
-(* -------------- semantic functions ---------------- *)
+(* -------------- atomic expressions  ---------------- *)
 
 Definition evalPrim (p : PrimOp) : value  := 
   match p with 
@@ -49,7 +49,7 @@ Definition evalPrim (p : PrimOp) : value  :=
   | common.IsInt => Prim.isInt
   | common.IsArr => Prim.isArr
   | common.IsFun => Prim.isFun
-  | _ => Dom.Int 0  (* others.... *)
+  | _ => Dom.Int 0  (* others primitives *)
   end.
 
 (* Evaluation function for simple values. 
@@ -63,7 +63,7 @@ Fixpoint evalA (e : mini.Expr) (ρ : env) : value :=
   | _ => Dom.Int 0
   end.
 
-(* ------------- operations on sequences of sets ---------------- *)
+(* ------- operations on sequences of sets ---------- *)
 
 
 Definition SUCCEED {A} : list (P A) := [ Total_set ]. 
@@ -78,7 +78,11 @@ Definition UNIFY {A} (d1 : list (P A)) (d2: list (P A)) : list (P A) :=
   ρ2 <- d2 ;;
   [ ρ1 ∩ ρ2 ].
 
-Infix "*" := UNIFY.
+Definition MINUS {A} (d1 : list (P A)) (d2: list (P A)) : 
+  list (P A) := 
+  ρ1 <- d1 ;;
+  ρ2 <- d2 ;;
+  [ @Setminus A ρ1 ρ2 ].
 
 
 (* left to right squash *)
@@ -125,6 +129,59 @@ Proof.
 Qed.
 
 
+(* dodgy union *)
+(* elementwise union of sequences, missing elements are ∅s.  *)
+Fixpoint unions {A} (VS : list (P A)) (WS : list (P A)) : 
+  list (P A) := 
+  match VS , WS with 
+  | [] , _ => WS
+  | _  , [] => VS 
+  | V :: VS', W :: WS' => (V ∪ W) :: unions VS' WS' 
+  end.
+
+Definition Unions {A} : list (list (P A)) -> list (P A) :=
+  List.fold_right unions nil.         
+
+(* every position in VS contains corresponding 
+   elements from VVS *)
+Definition UNIONS : P (list VAL) -> P (list VAL) := 
+  fun (VVS : list VAL -> Prop) (VS : list VAL) => 
+    forall V i, 
+      List.nth_error VS i = Some V -> 
+      V = fun (v : value) => 
+          exists (WS : list VAL) W, 
+            (WS ∈ VVS) /\
+            List.nth_error WS i = Some W /\
+            (v ∈ W).
+
+Definition ONE {A} (VS : list (P A)) : P A := 
+  let start := ∅ in
+  let step := fun xs x => x in
+  squash_fold_left step VS start.
+
+Example ONE_example_none {A} : @ONE A  [ ∅ ] = ∅ .
+  eapply Extensionality_Ensembles. split.
+  - move => y yIn. 
+    destruct yIn as [[h1 h2]|h1]. 
+    auto. destruct h1; auto.
+  - move => y yIn. done.
+Qed.
+
+Example ONE_example {A} (x:A) : ONE  [ ∅ ; ⌈ x ⌉ ] = ⌈ x ⌉.
+Proof.
+  eapply Extensionality_Ensembles. split.
+  - move => y yIn. 
+    destruct yIn as [[h1 h2]|h1].
+    eapply not_Singleton_empty; eauto.
+    destruct h1 as [_ h2]. done.
+  - move => y yIn.
+    right.
+    split. intro h. eapply not_Singleton_empty; eauto. auto.
+Qed.
+
+
+
+
 (* -------------- auxiliary definitions for VAL ------ *)
 
 (* Create a tuple from a list of VALs *)
@@ -133,8 +190,9 @@ Definition tups (VS : list VAL) : VAL :=
     exists (vs : list value), 
       v = mkTup vs /\ List.Forall2 Sets.In vs VS.
 
-(* apply f to x. 
-   F is a list of partial functions, corresponding to 
+(* apply f to x 
+
+   f is a list of partial functions, corresponding to 
    iteration on the input. Any inputs that are in the 
    domain of the function will produce output.
  *)
@@ -149,17 +207,20 @@ Definition apply (f : value) (v : value) : list VAL :=
   | _ => []
   end.
 
+Example apply_tup0 x y : apply (mkTup [x;y]) (Int 0) = [ ⌈ x ⌉ ; ∅ ]. cbn. auto. Qed.
+Example apply_tup1 x y : apply (mkTup [x;y]) (Int 1) = [ ∅ ; ⌈ y ⌉ ]. cbn. auto. Qed.
+Example apply_add1 : apply Prim.add1 (Int 0) = [ ⌈ Int 1 ⌉ ]. cbn. auto. Qed.
+Example apply_isInt : apply Prim.isInt (Int 1) = [ ⌈ Int 1 ⌉ ]. cbn. auto. Qed.
   
 (* ---------- auxiliary definitions for ENV and list ENV ------ *)
 
-(* destinguished result variable *)
+(* destinguished result variable (0) *)
 Definition r : Ident := mini.Test.r.
 
 (* Constrain a variable to be equal to a particular value.
    All other mappings in the environment are unconstrained. *)
 Definition constrain (x : Ident) (f : env -> value) : ENV := 
   fun ρ => ρ x = f ρ.
-
 
 (* Generalize all of the xs to be anything *)
 (* "Envs Drop Variables" *)
@@ -178,7 +239,7 @@ Definition hide_list (xs : Scope.t) (Δs : list ENV) : list ENV :=
 Definition envs_difference (es : ENV) (xs : Scope.t) (fs : ENV) : ENV := 
   e <- es ;;
   f <- fs ;;
-  guard (not (e ∈ (hide xs ⌈f⌉))) ⌈ e ⌉.
+  when (not (e ∈ (hide xs ⌈f⌉))) ⌈ e ⌉.
 
 
 (* Two different versions of application. Arguments must be atomic, 
@@ -202,7 +263,6 @@ Definition APP (e1 : mini.Expr) (e2 : mini.Expr) : list ENV :=
   [ APPi e1 e2 i ].
 
 
-
 (* find all environments in Δ such that ρ(r) = v and then hide r *)
 Definition extract (Δ : ENV) : P (value * ENV) := 
   fun '(v , Δ'') => 
@@ -219,18 +279,80 @@ Definition ALL (s : list ENV) : ENV :=
   '( vs, Δ ) <- combine s ;;
      (Δ ∩ (constrain r (fun _ => mkTup vs))).
 
+
+(* Find the first nonempty set in the sequence, if there is
+   one. *)
+(*
+Fixpoint ONE (xs: list ENV) : ENV := 
+  match xs with 
+  | nil => ∅
+  | x :: xs' => fun ρ => 
+        (x = ∅ /\ (ρ ∈ ONE xs')) \/
+        (x <> ∅ /\ (ρ ∈ x ))
+  end.
+
+Example ONE_s s : ONE [ ∅ ; s ; ∅ ] = s.
+cbv. eapply Extensionality_Ensembles.
+split.    
+- intros ρ [[h1 [[h3 h5]| h4]]| h2].
+  + destruct h5. destruct H. subst. auto. destruct H.
+    done.
+  + destruct h4. done.
+  + destruct h2. done.
+- intros ρ h. 
+  cbv. left. split; auto.
+  right. split. intro h1. subst. done. done.
+Qed.
+*)
+
+
+
+
+(* The set of all environments that extend rho with arbitrary 
+   definitions for the variables declared in e. 
+   Is this the same as "hide (mini.I e) ⌈ ρ ⌉"
+
+*)
+
+Definition X (e : mini.Expr) (ρ : env) : ENV :=
+  hide (mini.I e) ⌈ ρ ⌉.
+(*
+  fun rho' =>
+    forall x, 
+      if (Scope.mem x (mini.I e)) 
+      then exists v, rho' x = v    (* arbitrary value for vars in new scope *)
+      else rho' x = rho x.         (* same value for vars in old scope *)
+*)
+
+
+Definition SEQ (d1 : list ENV) (d2: list ENV) : list ENV := 
+  UNIFY (hide_list (Scope.singleton r) d1) d2.
+
+
 (* ------  Notation ----------------------------------------- *)
 
+Infix "⩅" := unions (at level 70).
 Infix "≈" := constrain (at level 60).
 Notation "Δ \ xs" := (hide xs Δ) (at level 70).
 Notation "Δ [\] xs" := (hide_list xs Δ) (at level 70).
-Notation "es \{ xs } fs" := (envs_difference es xs fs) (at level 40) : ENV_scope.
-
+Notation "es \{ xs } fs" := (envs_difference es xs fs) (at level 40).
 Notation "⟨ n ⟩" := (fun ρ => Int n) (at level 40).
+Infix "*" := UNIFY.
 
-Lemma extend_lookup_same {x ρ v} : (x |-> v, ρ) x = v. Admitted.
+
+(* ------  Some theory ----------------------------------------- *)
+
 Lemma not_r : forall (x r : Ident), (SetoidList.InA eq x [r] -> False) -> Nat.eqb r x = false. Admitted.
-Lemma extend_lookup_diff {x y ρ v} : Nat.eqb x y = false -> (x |-> v, ρ) y = ρ y. Admitted.
+
+Lemma hide_intersect x s1 s2 : hide x (s1 ∩ s2) ⊆ ((hide x s1) ∩ (hide x s2)).
+Proof. 
+  intros ρ [_ [[ρ' h11] h2]].
+  unfold hide.
+    split. 
+    exists ρ'. split; auto. exists ρ'. split; auto.
+Qed. 
+(* NOTE: converse is not true *)
+
 
 Lemma hide_constraint {i v} : (i ≈ fun _ => v) \ (Scope.singleton i) ≃ Total_set.
 split. 
@@ -243,12 +365,38 @@ intros x NI.
 apply not_r in NI. rewrite extend_lookup_diff; auto.
 Qed.
 
+Lemma hide_all s : (hide s Total_set) = Total_set.
+  eapply Extensionality_Ensembles.
+  split.
+  intros x xIn. cbv. auto.
+  intros x xIn. unfold hide.
+  exists x. split. auto.
+  intros y IH. auto.
+Qed.
+
+
 Lemma extract_one {x} : extract (r ≈ ⟨ x ⟩) = ⌈(Int x, Total_set)⌉.
 eapply Extensionality_Ensembles.
+unfold extract. unfold hide_r. 
 split.
 - intros [v ρ] yIn. 
   cbn in yIn.
+  have: ρ ≃ Total_set.  split. intros z zIn. cbv. auto.
+  intros z _. rewrite yIn.
+  cbv. 
 Admitted.  
+
+Lemma SEQ_SUCCEED_X X : SEQ SUCCEED X = X.
+  unfold SEQ, UNIFY, hide_list, SUCCEED.
+  cbn.
+  rewrite hide_all.
+  rewrite List.app_nil_r.
+  induction X.
+  - cbn. auto.
+  - cbn. f_equal.
+    eapply all_intersect.
+    auto.
+Qed.
 
 Example ex_ALL : 
   (r |-> mkTup [Int 3;Int 4]) ∈ (ALL [ r ≈ ⟨3⟩;  r ≈ ⟨4⟩] ).
@@ -268,7 +416,17 @@ Admitted.
 
 Module DLS.
 
+
 Fixpoint E (e : mini.Expr) : list ENV := 
+
+  let B (e : mini.Expr) :list ENV := 
+    Δ <- E e ;;
+    [ Δ \ mini.I e ] in
+
+  let V (e : mini.Expr) : list (P (value * ENV)) := 
+    Δ <- B e ;;
+    [ extract Δ ] in
+
   match e with 
   | mini.DefineV _ => [ Total_set ]
 
@@ -277,27 +435,31 @@ Fixpoint E (e : mini.Expr) : list ENV :=
   | mini.EPrim _ => [ r ≈ evalA e ]
   | mini.Array es =>  [ r ≈ evalA e ]
 
-  | mini.Fail => FAIL 
+  | mini.Fail => FAIL   (* or [] ? *)
 
   | mini.Choice e1 e2 => E e1 ++ E e2
 
-  | mini.Seq e1 e2 => (E e1 [\] Scope.singleton r) * E e2
+  | mini.Seq e1 e2 => SEQ (E e1) (E e2)
 
-  | mini.Unify e1 e2 => E e1 * E e2
+  | mini.Unify e1 e2 => E e1 * E e2  (* missing from fig *)
 
   | mini.ApplyD e1 e2 => APP e1 e2
 
   | mini.If3 a b c =>  
-    (* Note, not quite right *)
+
     let Y := mini.I a in 
-    ((E a [\] (Scope.add r Y)) * (E b [\] Y)) ++ (E c [\] Y)
+    let rY := Scope.add r Y in
+
+     ((E a [\] rY) * (E b [\] Y)) ⩅
+     (MINUS (E c) (E a [\] Y))
 
   | mini.All a => 
-      let Y := mini.I a in 
-      [ ALL (E a) ] 
-      
+      [ ALL (E a) \ mini.I a ] 
 
-  (* TODO: functions, all, one *)                                                    
+  | mini.One a => 
+      [ ONE (E a) \ mini.I a ]
+
+  (* TODO: functions *)
 
   | _ => [ ∅ ] 
   end.
@@ -308,43 +470,13 @@ End DLS.
 
 Module DSLS.
 
-
-
-
-(* Semantic operations *)
-
-Definition HIDE (xs : Scope.t) (DS : list ENV) : list ENV := 
-  hide xs <$> DS.
-
-
-Definition r : Ident := mini.Test.r.
-
-Definition hide_r : ENV -> ENV := hide (Scope.singleton r).
-
-(* find all environments in Δ such that ρ(r) = v and then hide r *)
-Definition extract (Δ : ENV) : P (value * ENV) := 
-  fun '(v , Δ'') => 
-    Δ'' = hide_r (Δ ∩ (r ≈ (fun _ => v))).
-
-Definition combine : list ENV -> P (list value * ENV) := 
-  List.fold_right 
-    (fun Δ VSS => 
-       '(vi, Δi) <- extract Δ ;;
-       fun '(vs, Δs) => (vi :: vs, Δi ∩ Δs) ∈ VSS)
-    (fun _ => False).
-       
-Definition ALL (s : list ENV) : list ENV := 
-  [ '( vs, Δ ) <- combine s ;;
-     (Δ ∩ (r ≈ (fun _ => mkTup vs))) ].
-  
-Definition SEQ (d1 : list ENV) (d2: list ENV) : list ENV := 
-  UNIFY (HIDE (Scope.singleton r) d1) d2.
-
+Definition map2 {A B} : (A -> B) -> (P (list A)) -> (P (list B)) := 
+  fun f => fmap (fmap f).
 
 Fixpoint E (e : mini.Expr) : P (list ENV) := 
 
   let B (e : mini.Expr) : P (list ENV)  :=
-    HIDE (mini.I e) <$> (E e)
+    (fmap (hide (mini.I e))) <$> (E e)
   in
 
   match e with 
@@ -362,14 +494,14 @@ Fixpoint E (e : mini.Expr) : P (list ENV) :=
 
   | mini.Fail => ⌈ FAIL ⌉
 
-  | mini.Choice e1 e2 => CHOICE <$> (B e1) <*> (B e2)
+  | mini.Choice e1 e2 => CHOICE <$> B e1 <*> B e2
 
-  | mini.Seq e1 e2 => SEQ <$> (E e1) <*> (E e2)
+  | mini.Seq e1 e2 => SEQ <$> E e1 <*> E e2
 
-  | mini.Unify e1 e2 => UNIFY <$> (E e1) <*> (E e2)
-
-  | mini.All e1 => ALL <$> (B e1)
-
+  | mini.Unify e1 e2 => UNIFY <$> E e1 <*> E e2
+(* 
+  | mini.All e1 => (fun x => [ ALL x ]) <$> (B e1)
+*)
   | mini.If3 e1 e2 e3 => fun _ => False
       
   | mini.Fun q eff i e1 (y,h,x) e2 => fun _ => False
@@ -378,46 +510,10 @@ Fixpoint E (e : mini.Expr) : P (list ENV) :=
 
   end.
 
-Lemma hide_all s : (hide s Total_set) = Total_set.
-  eapply Extensionality_Ensembles.
-  split.
-  intros x xIn. cbv. auto.
-  intros x xIn. unfold hide.
-  exists x. split. auto.
-  intros y IH. auto.
-Qed.
+(* ---------------------------------------------------- *)
 
-
-Lemma all_intersect {A} (s : P A) : (Total_set ∩ s) = s.
-Proof.
-  eapply Extensionality_Ensembles.
-  split. intros x xIn. inversion xIn. auto.
-  split. cbv. auto. auto.
-Qed.
-
-Lemma intersect_all {A} (s : P A) : (s ∩ Total_set) = s.
-  eapply Extensionality_Ensembles.
-  split. intros x xIn. inversion xIn. auto.
-  split; cbv; auto. 
-Qed.
-
-Lemma in_singleton' {A} (x y : A) : x = y -> x ∈ ⌈ y ⌉.
-Proof. intros. subst. eapply in_singleton. Qed.
-
-Lemma SEQ_SUCCEED_X X : SEQ SUCCEED X = X.
-  unfold SEQ, UNIFY, HIDE, SUCCEED.
-  cbn.
-  rewrite hide_all.
-  rewrite List.app_nil_r.
-  induction X.
-  - cbn. auto.
-  - cbn. f_equal.
-    eapply all_intersect.
-    auto.
-Qed.
 
 Definition x : Ident := mini.Test.x.
-
 
 
 (* { x:=1; x }  *)
@@ -452,7 +548,7 @@ Proof.
     eexists.
     split.
     eapply in_singleton.
-    unfold SEQ, UNIFY, HIDE.
+    unfold SEQ, UNIFY, hide.
     cbn.
     eapply in_singleton'.
     f_equal.
@@ -496,6 +592,118 @@ End DSLS.
 (* -------------------------------------------------------- *)
 (* -------------------------------------------------------- *)
 (* -------------------------------------------------------- *)
+
+Module ELV.
+
+Definition ALL (VS : list VAL) : VAL := 
+  let start := ⌈ mkTup [] ⌉ in
+  squash_fold_left (liftM2 snoc) VS start.
+
+Lemma snoc_mktup xs v : 
+  snoc (mkTup xs) v = mkTup (xs ++ [v]).
+Admitted.
+
+Example ALL_example : 
+  ALL [ ⌈ Int 2 ⌉ ; ⌈ Int 3 ⌉ ] = ⌈ mkTup [Int 2; Int 3] ⌉.
+cbn. eapply Extensionality_Ensembles. split.
+- move => x [[h1 [[h2 h3]|h2]]|h1]. 
+  eapply not_Singleton_empty; eauto.
+  eapply not_Singleton_empty; eauto.
+  destruct h1 as [_ [a h1]].
+  destruct h1 as [[h1|h3] [v [h2 h4]]].
+  destruct h1.
+  eapply not_Singleton_empty; eauto.
+  destruct h3 as [_ [b [h5 [c [h6 h7]]]]].
+  inversion h6. inversion h2. subst. inversion h5. subst.
+  inversion h7. subst.
+  rewrite snoc_mktup in h4.
+  rewrite snoc_mktup in h4.
+  cbn in h4. eauto.
+- admit.
+Admitted.
+
+
+(* TODO(!!): this is not correct as it doesn't filter out 
+   the empty sets of the sequence. *)
+Definition SEQ (s1 : list VAL) (s2 : list VAL) : list VAL := 
+  v1 <- s1 ;; s2.
+  
+
+(* another version of the dodgy big union *)
+Definition UNIONS (VVS : P (list VAL)) : list VAL := 
+  i <- allNums ;;
+  let V := ( VS <- VVS ;; List.nth i VS ∅ ) in
+  [ V ].
+
+
+Fixpoint E (e :mini.Expr) (ρ:env) : list VAL := 
+  
+  let B (e : mini.Expr) (ρ : env) : list VAL  := 
+    UNIONS
+      (ρ' <- X e ρ ;; ⌈ E e ρ' ⌉) 
+    in
+  let R (e : mini.Expr) ρ : ENV := 
+    ρ' <- X e ρ ;; 
+    when (E e ρ' <> []) 
+    ⌈ ρ' ⌉
+  in
+
+  match e with 
+
+  | mini.Block e =>  B e ρ
+
+  | mini.Var _ => [ ⌈evalA e ρ⌉ ]
+  | mini.Lit _ => [ ⌈evalA e ρ⌉ ] 
+  | mini.EPrim _ => [ ⌈evalA e ρ⌉ ] 
+  | mini.Array es =>  [ ⌈evalA e ρ⌉ ] 
+
+  | mini.DefineV _ => [ ⌈ mkTup[] ⌉ ]
+
+  | mini.ApplyD e1 e2 => apply (evalA e1 ρ) (evalA e2 ρ)
+
+  | mini.Fail => [∅]
+
+  | mini.Choice e1 e2 => CHOICE (B e1 ρ) (B e2 ρ)
+
+  | mini.Seq e1 e2 => SEQ (E e1 ρ) (E e2 ρ)
+
+  | mini.Unify e1 e2 => UNIFY (E e1 ρ) (E e2 ρ)
+
+  | mini.All e1 =>  [ ALL (B e1 ρ) ]
+
+  | mini.If3 e1 e2 e3 => 
+      let Δ  : ENV := R e1 ρ in
+      let TS := UNIONS ( ρ' <- Δ ;; ⌈ B e2 ρ' ⌉ )in
+      let FS := B e2 ρ in
+      (* TODO: combine these together better *)
+      TS ++ FS
+      
+  | mini.Fun q eff i e1 (y,h,x) e2 =>  []
+
+  | _ => []
+
+  end.
+
+End ELV.
+
+(* -------------------------------------------------------- *)
+
+Lemma Equiv1 (e : mini.Expr) (ρ : env) : 
+  ELV.E e ρ = 
+    Δ <- DLS.E e ;;
+    [ '(v, Δ') <- extract Δ ;;
+         when (ρ ∈ Δ') ⌈v⌉ ].
+Admitted.
+
+Lemma Equiv2 (e : mini.Expr) : 
+  DLS.E e = 
+    i <- allNums ;;
+    [ ρ <- Total_set ;;
+      let VS := ELV.E e ρ in
+      when (ρ r ∈ List.nth i VS ∅) 
+      ⌈ ρ ⌉ ].
+Admitted.  
+
 
 (* -------------- Squash ------------ *)
 
@@ -560,47 +768,6 @@ Definition TailSquash {A} : list (P A) -> list (P A) -> Prop :=
   fun VS WS => 
     (exists n, VS = WS ++ List.repeat ∅ n) /\ NonEmptyTail WS.
 
-(* ---------- Extended environments for blocks ------------ *)
-
-
-(* The set of all environments that extend rho with arbitrary 
-   definitions for the variables declared in e. 
-
-*)
-
-Definition X (e : mini.Expr) (rho : env) : ENV :=
-  fun rho' =>
-    forall x, 
-      if (Scope.mem x (mini.I e)) 
-      then exists v, rho' x = v    (* arbitrary value for vars in new scope *)
-      else rho' x = rho x.         (* same value for vars in old scope *)
-
-
-(* --------- (dodgy) unions ------------ *)
-         
-(* elementwise union of sequences, missing elements are ∅s.  *)
-Fixpoint unions {A} (VS : list (P A)) (WS : list (P A)) : 
-  list (P A) := 
-  match VS , WS with 
-  | [] , _ => WS
-  | _  , [] => VS 
-  | V :: VS', W :: WS' => (V ∪ W) :: unions VS' WS' 
-  end.
-
-Definition Unions {A} : list (list (P A)) -> list (P A) :=
-  List.fold_right unions nil.
-
-(* every position in VS contains corresponding 
-   elements from VVS *)
-Definition UNIONS : P (list VAL) -> P (list VAL) := 
-  fun (VVS : list VAL -> Prop) (VS : list VAL) => 
-    forall V i, 
-      List.nth_error VS i = Some V -> 
-      V = fun (v : value) => 
-          exists (WS : list VAL) W, 
-            (WS ∈ VVS) /\
-            List.nth_error WS i = Some W /\
-            (v ∈ W).
 
 Lemma UNIONS_mem (ls : list (list VAL)) : (UNIONS (mem ls)) = ⌈ Unions ls ⌉.
 Proof.
@@ -608,6 +775,10 @@ Admitted.
 
 
 (* ----------------- version: fixpoint ----------- *)
+
+
+
+
 
 Module FixpointVersion.
 
@@ -1017,6 +1188,7 @@ Proof. unfold mini.Test.t2.
        - subst.
          exists (mini.Test.x |-> Dom.Int 1 ).
          split; auto.
+(*
          ++ intros y.
             destruct Scope.mem eqn:IN.
             -- (* in new scope *) 
@@ -1033,7 +1205,7 @@ Proof. unfold mini.Test.t2.
               admit.
               admit.
          ++ eeval.
-       - done.
+       - done. *)
 Admitted.
 
 
