VerseRocq/verse/densem/tenv.v
@@ -3,6 +3,7 @@ Require Import Imports.
 From Stdlib Require Lists.List.
 From Stdlib Require Import Classes.EquivDec.
 From Stdlib Require Export FunctionalExtensionality.
+From Stdlib Require Import PeanoNat.
 
 Import ssreflect.
 
@@ -48,16 +49,36 @@ Notation " x |-> v " := (Env.extend x v Env.empty) (at level 80) : env_scope.
 Notation " x |-> v , e " := (Env.extend x v e) (at level 80, right associativity): env_scope. 
 End EnvNotation.
 
+Open Scope env_scope.
+Import EnvNotation.
+
+Section NotationTest.
+Variable x : Ident.
+Variable y : Ident.
+Check (x |-> Int 3, y |-> Int 4).
+End NotationTest.
+
+Create HintDb env.
+
+Lemma Extensionality_env (ρ1 ρ2 : env) : 
+  (forall x, ρ1 x = ρ2 x) -> ρ1 = ρ2.
+Proof. intros. extensionality y. auto. Qed.
 
 Lemma empty_equal r:
-  (forall x, r x = Dom.Int 0) -> 
-  Env.empty = r.
+  (forall x, r x = Int 0) -> 
+  r = Env.empty.
 Proof. 
   intro h.
   extensionality x.
   rewrite h.
   auto.
 Qed.
+
+
+Lemma extend_lookup_same {x ρ v} : (x |-> v, ρ) x = v. unfold Env.extend. rewrite Nat.eqb_refl. auto. Qed.
+
+Lemma extend_lookup_diff {x y ρ v} : Nat.eqb x y = false -> (x |-> v, ρ) y = ρ y. 
+  unfold Env.extend. destruct (x =? y). intro h; try done. intro h. done. Qed.
 
 Lemma extend_equal r s x v:
   s x = v -> (forall y, Nat.eqb x y = false -> r y = s y) ->
